Factoring out OpenT
- It remains specialized because otherwise it costs
  extra performance.

theories/Lambda/ExprDI.v
@@ -1,5 +1,7 @@
 Require Import ExtLib.Core.RelDec.
 Require Import ExtLib.Structures.Monads.
+Require Import ExtLib.Structures.Applicative.
+Require Import ExtLib.Structures.Functor.
 Require Import ExtLib.Data.HList.
 Require Import ExtLib.Data.List.
 Require Import ExtLib.Data.Fun.
@@ -9,6 +11,7 @@ Require Import MirrorCore.EnvI.
 Require Import MirrorCore.SymI.
 Require Import MirrorCore.ExprI.
 Require Import MirrorCore.Lambda.TypesI2.
+Require Import MirrorCore.Lambda.ResType.
 Require Import MirrorCore.Lambda.ExprCore.
 
 Set Implicit Arguments.
@@ -55,66 +58,20 @@ Module Type ExprDenote.
     : forall {ts a b} (pf : Rty ts a b), typD ts a -> typD ts b :=
       @Rcast (fun T => T).
 
-    Section OpenT.
-      Variable ts : list Type.
-      Variables tus tvs : tenv typ.
+    Definition OpenT ts := ResType.OpenT (typD ts).
+    Definition Open_UseV := ResType.Open_UseV.
+    Definition Open_UseU := ResType.Open_UseU.
+    Definition Open_Inj ts tus tvs := Eval simpl in @pure (OpenT ts tus tvs) _.
 
-      Definition OpenT (T : Type) :=
-        hlist (typD ts) tus -> hlist (typD ts) tvs -> T.
-
-      Definition Open_UseV (n : nat) : option { t : typ & OpenT (typD ts t) } :=
-        bind (m := option)
-             (nth_error_get_hlist_nth _ tvs n)
-             (fun t_get =>
-                let '(existT t get) := t_get in
-                ret (@existT _ (fun t => OpenT (typD ts t)) t
-                             (fun us vs => get vs))).
-
-      Definition Open_UseU (n : nat) : option { t : typ & OpenT (typD ts t) } :=
-        bind (m := option)
-             (nth_error_get_hlist_nth _ tus n)
-             (fun t_get =>
-                let '(existT t get) := t_get in
-                ret (@existT _ (fun t => OpenT (typD ts t)) t
-                             (fun us vs => get us))).
-
-      Definition Open_App {t u}
-      : OpenT (typD ts (typ_arr t u)) -> OpenT (typD ts t) -> OpenT (typD ts u) :=
-        match eq_sym (typD_arr ts t u) in _ = T
-              return OpenT T -> OpenT (typD ts t) -> OpenT (typD ts u)
-        with
-          | eq_refl => fun f x => fun us vs => (f us vs) (x us vs)
-        end.
-
-      Definition Open_Inj {t} (val : typD ts t)
-      : OpenT (typD ts t) :=
-        fun _ _ => val.
-
-
-      (** Auxiliary definitions **)
-      Definition Open_GetUAs (n : nat) (t : typ) :
-        option (OpenT (typD ts t)) :=
-        bind (m := option)
-             (nth_error_get_hlist_nth (typD ts) tus n)
-             (fun t_get =>
-                let '(existT t' get) := t_get in
-                bind (m := option)
-                     (type_cast ts t' t)
-                     (fun cast =>
-                        ret (fun us vs => Rcast_val cast (get us)))).
-
-      Definition Open_GetVAs (n : nat) (t : typ) :
-        option (OpenT (typD ts t)) :=
-        bind (m := option)
-             (nth_error_get_hlist_nth (typD ts) tvs n)
-             (fun t_get =>
-                let '(existT t' get) := t_get in
-                bind (m := option)
-                     (type_cast ts t' t)
-                     (fun cast =>
-                        ret (fun us vs => Rcast_val cast (get vs)))).
-
-    End OpenT.
+    Definition Open_App {ts tus tvs t u}
+    : OpenT ts tus tvs (typD ts (typ_arr t u)) -> OpenT ts tus tvs (typD ts t) -> OpenT ts tus tvs (typD ts u) :=
+      match eq_sym (typD_arr ts t u) in _ = T
+            return OpenT ts tus tvs T ->
+                   OpenT ts tus tvs (typD ts t) ->
+                   OpenT ts tus tvs (typD ts u)
+      with
+        | eq_refl => fun f x => fun us vs => (f us vs) (x us vs)
+      end.
 
     Definition Open_Abs {ts tus tvs t u}
     : OpenT ts tus (t :: tvs) (typD ts u) ->
@@ -124,7 +81,6 @@ Module Type ExprDenote.
       with
         | eq_refl => fun f => fun us vs x => f us (Hcons x vs)
       end.
-
 
     Definition funcAs {ts} (f : func) (t : typ) : option (typD ts t) :=
       match typeof_sym f as Z
