theories/Lambda/ResType.v
@@ -1,0 +1,71 @@
+Require Import Coq.Relations.Relations.
+Require Import Coq.Classes.Morphisms.
+Require Import ExtLib.Structures.Monad.
+Require Import ExtLib.Structures.Applicative.
+Require Import ExtLib.Structures.Functor.
+Require Import ExtLib.Data.HList.
+Require Import ExtLib.Data.List.
+Require Import MirrorCore.EnvI.
+
+Set Implicit Arguments.
+Set Strict Implicit.
+
+Section OpenT.
+  Variable typ : Type.
+  Variable typD : typ -> Type.
+  Variables tus tvs : tenv typ.
+
+  Definition OpenT (T : Type) :=
+    hlist typD tus -> hlist typD tvs -> T.
+
+  Global Instance Applicative_OpenT : Applicative OpenT :=
+  { pure := fun _ val _ _ => val
+  ; ap := fun _ _ f x us vs => (f us vs) (x us vs)
+  }.
+
+  Global Instance Functor_OpenT : Functor  OpenT :=
+  { fmap := fun _ _ f x => fun us vs => (f (x us vs)) }.
+
+  Definition Open_UseU (n : nat) : option { t : typ & OpenT (typD t) } :=
+    match nth_error_get_hlist_nth _ tus n with
+      | None => None
+      | Some (existT t get) =>
+        Some (@existT _ (fun t => OpenT (typD t)) t (fun us _ => get us))
+    end.
+
+  Definition Open_UseV (n : nat) : option { t : typ & OpenT (typD t) } :=
+    match nth_error_get_hlist_nth _ tvs n with
+      | None => None
+      | Some (existT t get) =>
+        Some (@existT _ (fun t => OpenT (typD t)) t (fun _ => get))
+    end.
+
+  Definition OpenTeq T (R : relation T) : relation (OpenT T) :=
+    fun a b => forall x y, R (a x y) (b x y).
+
+  Theorem pure_eq
+  : forall T (R : relation T) a b, R a b -> OpenTeq R (pure a) (pure b).
+  Proof. compute; intros; assumption. Qed.
+
+  Theorem ap_eq
+  : forall T U (Rt : relation T) (Ru : relation U) f g a b,
+      OpenTeq (Rt ==> Ru)%signature f g -> OpenTeq Rt a b ->
+      OpenTeq Ru (ap f a) (ap g b).
+  Proof. compute. auto. Qed.
+
+  Theorem fmap_eq
+  : forall T U (Rt : relation T) (Ru : relation U) f g a b,
+      (Rt ==> Ru)%signature f g -> OpenTeq Rt a b ->
+      OpenTeq Ru (fmap f a) (fmap g b).
+  Proof. compute; auto. Qed.
+
+End OpenT.
+
+Section OpenT_Abs.
+  Variable typ : Type.
+  Variable typD : typ -> Type.
+
+  Definition Open_Abs {tus tvs t T} (f : OpenT typD tus (t :: tvs) T)
+  : OpenT typD tus tvs (typD t -> T) :=
+    fun us vs x => f us (Hcons x vs).
+End OpenT_Abs.
